Universe-generalize completeness thm

equational_theories/FreeMagma.lean
@@ -1,6 +1,7 @@
 import equational_theories.AllEquations
 import equational_theories.EquationalResult
 import equational_theories.Homomorphisms
+import Mathlib.Data.List.NodupEquivFin
 
 universe u
 universe v
@@ -29,19 +30,56 @@ instance FreeMagma.isMagma {α} : Magma (FreeMagma α) := ⟨ Fork ⟩
 
 namespace FreeMagma
 
-def evalInMagma {α : Type u} {G : Type v} [Magma G] (f : α -> G) : FreeMagma α → G
+def evalInMagma {α : Type u} {G : Type v} [Magma G] (f : α → G) : FreeMagma α → G
   | Lf a => f a
-  | lchild ⋆ rchild => (evalInMagma f lchild) ◇ (evalInMagma f rchild)
+  | lchild ⋆ rchild => evalInMagma f lchild ◇ evalInMagma f rchild
 
 def evalHom {α : Type u} {G : Type v} [Magma G] (f : α → G) : FreeMagma α →◇ G where
    toFun := evalInMagma f
    map_op' := fun _ _ ↦ refl _
+
+@[simp] theorem evalHom_apply {α G} [Magma G] (f : α → G) (m : FreeMagma α) :
+    evalHom f m = evalInMagma f m := rfl
+
+theorem evalInMagma_leaf {α} (m : FreeMagma α) : evalInMagma Lf m = m := by
+  induction m <;> simp [evalInMagma, *]
 
  def fmapFreeMagma {α : Type u} {β : Type v} (f : α → β) : FreeMagma α → FreeMagma β :=
     evalInMagma (Lf ∘ f)
 
  def fmapHom {α : Type u} {β : Type v} (f : α → β) : FreeMagma α →◇ FreeMagma β :=
    evalHom (Lf ∘ f)
+
+theorem evalInMagma_hom {α G H} [Magma G] [Magma H] (f : α → G) (g : G →◇ H) (m : FreeMagma α) :
+    g (evalInMagma f m) = evalInMagma (g ∘ f) m := by
+  induction m <;> simp [evalInMagma, g.map_op, *]
+
+theorem evalInMagma_equiv {α G H} [Magma G] [Magma H] (f : α → G) (g : G ≃◇ H) (m : FreeMagma α) :
+    g (evalInMagma f m) = evalInMagma (g ∘ f) m :=
+  evalInMagma_hom f (MagmaHomClass.toMagmaHom g) m
+
+theorem SubstEval {α β G} [Magma G] (t : FreeMagma α) (σ : α → FreeMagma β) (φ : β → G) :
+    evalInMagma φ (evalInMagma σ t) = evalInMagma (evalInMagma φ ∘ σ) t :=
+  evalInMagma_hom _ (evalHom _) _
+
+theorem evalInMagma_fmapHom {α β G} [Magma G] (f : α → β) (g : β → G) (m : FreeMagma α) :
+    evalInMagma g (fmapHom f m) = evalInMagma (g ∘ f) m := by
+  show evalInMagma g (evalInMagma (Lf ∘ f) m) = evalInMagma (g ∘ f) m
+  induction m <;> simp [evalInMagma, *]
+
+theorem evalHom_comp_fmapHom {α β G} [Magma G] (f : α → β) (g : β → G) :
+    (fmapHom f).comp (evalHom g) = evalHom (g ∘ f) := by
+  ext m; apply evalInMagma_fmapHom
+
+theorem fmapHom_comp' {α β γ} (f : α → β) (g : β → γ) (m : FreeMagma α) :
+    fmapHom g (fmapHom f m) = fmapHom (g ∘ f) m := by
+  rw [fmapHom, evalHom_apply, evalInMagma_fmapHom]; rfl
+
+theorem fmapHom_comp {α β γ} (f : α → β) (g : β → γ) :
+    (fmapHom f).comp (fmapHom g) = fmapHom (g ∘ f) := by
+  ext m; apply fmapHom_comp'
+
+theorem fmapHom_id {α} (m : FreeMagma α) : fmapHom id m = m := evalInMagma_leaf _
 
  theorem EvalFreeMagmaUniversalProperty {α : Type u} {G : Type v} [Magma G] (f : α → G)
     : ∀ g : FreeMagma α →◇ G, g.toFun ∘ Lf = f → evalInMagma f = g.toFun := by
@@ -58,6 +96,69 @@ def evalHom {α : Type u} {G : Type v} [Magma G] (f : α → G) : FreeMagma α �
  theorem FmapFreeMagmaUniversalProperty {α : Type u} [Magma α] {β : Type u} (f : α → β)
     : ∀ g : FreeMagma α →◇ FreeMagma β, g ∘ Lf = Lf ∘ f → fmapFreeMagma f = g :=
     EvalFreeMagmaUniversalProperty (Lf ∘ f)
+
+def Mem {α} (a : α) : FreeMagma α → Prop
+  | Lf a' => a = a'
+  | lchild ⋆ rchild => Mem a lchild ∨ Mem a rchild
+
+def first {α} : FreeMagma α → α
+  | Lf a => a
+  | lchild ⋆ _ => lchild.first
+
+theorem first_mem {α} : ∀ m : FreeMagma α, Mem m.first m
+  | Lf _ => rfl
+  | lchild ⋆ _ => .inl lchild.first_mem
+
+def elems {α} [DecidableEq α] : (m : FreeMagma α) → {l : List α // l.Nodup ∧ ∀ a, a ∈ l ↔ Mem a m}
+  | Lf a => ⟨[a], List.nodup_singleton _, by simp [Mem]⟩
+  | lchild ⋆ rchild => by
+    let ⟨l, _, hl⟩ := lchild.elems
+    let ⟨r, nr, hr⟩ := rchild.elems
+    use l ∪ r, .union _ nr; simp [Mem, hl, hr]
+
+def finEquiv {α} [DecidableEq α] (m : FreeMagma α) : Fin m.elems.1.length ≃ {a // Mem a m} := by
+  convert ← m.elems.2.1.getEquiv; apply m.elems.2.2
+
+def pmap {α β} : ∀ (m : FreeMagma α), (∀ a, Mem a m → β) → FreeMagma β
+  | Lf a, f => Lf (f a rfl)
+  | lchild ⋆ rchild, f =>
+    pmap lchild (fun a h => f a (.inl h)) ⋆ pmap rchild (fun a h => f a (.inr h))
+
+def attach {α} (m : FreeMagma α) : FreeMagma {a // Mem a m} := pmap m .mk
+
+def toFin {α} [DecidableEq α] (m : FreeMagma α) : FreeMagma (Fin m.elems.1.length) :=
+  fmapHom (finEquiv m).symm m.attach
+
+def toNat {α} [DecidableEq α] (m : FreeMagma α) : FreeMagma ℕ :=
+  fmapHom (·.val) (toFin m)
+
+theorem evalInMagma_pmap {α β G} [Magma G] {φ : β → G} {ψ : α → G}
+    (m : FreeMagma α) {f : (a : α) → Mem a m → β} (H : ∀ a h, φ (f a h) = ψ a) :
+    evalInMagma φ (m.pmap f) = evalInMagma ψ m := by
+  induction m <;> simp [pmap, evalInMagma, *]
+
+theorem attach_map_val {α} (m : FreeMagma α) : fmapHom (·.val) m.attach = m :=
+  (evalInMagma_pmap _ (by simp)).trans (fmapHom_id _)
+
+theorem mem_evalInMagma_of_mem {α β a b} {f : α → FreeMagma β} :
+    ∀ {m : FreeMagma α}, Mem b m → Mem a (f b) → Mem a (evalInMagma f m)
+  | Lf _, rfl, h => h
+  | _ ⋆ _, .inl h1, h2 => .inl <| mem_evalInMagma_of_mem h1 h2
+  | _ ⋆ _, .inr h1, h2 => .inr <| mem_evalInMagma_of_mem h1 h2
+
+theorem pmap_evalInMagma {α β γ} (f : α → FreeMagma β) (m : FreeMagma α)
+    (g : (a : β) → Mem a (evalInMagma f m) → γ)
+    (k : α → FreeMagma γ)
+    (h : ∀ a ha, ((f a).pmap fun b hb => g b (mem_evalInMagma_of_mem ha hb)) = k a) :
+    (evalInMagma f m).pmap g = evalInMagma k m := by
+  induction m with simp [evalInMagma, pmap, *]
+  | Leaf => exact h _ rfl
+  | Fork _ _ iha ihb => exact ⟨iha _ fun a ha => h a (.inl ha), ihb _ fun a ha => h a (.inr ha)⟩
+
+theorem pmap_eq_map {α β} (m : FreeMagma α)
+    (f : (a : α) → Mem a m → β) (g : α → β) (h : ∀ a h, f a h = g a) :
+    m.pmap f = fmapHom g m := by
+  simp [fmapHom]; induction m <;> simp [evalInMagma, pmap, *]
 
 end FreeMagma
 
