equational_theories/MagmaLaw.lean
@@ -5,7 +5,7 @@ open FreeMagma
 
 namespace Law
 
-structure MagmaLaw (α : Type) where
+structure MagmaLaw (α : Type*) where
   lhs : FreeMagma α
   rhs : FreeMagma α
 deriving DecidableEq
@@ -15,13 +15,6 @@ infix:60 " ≃ " => MagmaLaw.mk
 end Law
 
 open Law
-
-def substFreeMagma {α β} (t : FreeMagma α) (σ : α → FreeMagma β) : FreeMagma β :=
-match t with
-| .Leaf a => σ a
-| t₁ ⋆ t₂ => substFreeMagma t₁ σ ⋆ substFreeMagma t₂ σ
-
-infix:66 " ⬝ " => substFreeMagma
 
 @[inline, simp]
 def Ctx α := Set (MagmaLaw α)
@@ -41,92 +34,262 @@ local infix:50 " ⊢ " =>  derive
 
 -- We keep this in type, because we're going to want to gather
 -- the (finite!) set of required axioms later.
-/-- Definition for derivability-/
-inductive derive {α} : Ctx α → MagmaLaw α → Type :=
-  | Ax Γ E (h : E ∈ Γ) : Γ ⊢ E
-  | Ref Γ t : Γ ⊢ (t ≃ t)
-  | Sym Γ t u : Γ ⊢ (t ≃ u) → Γ ⊢ (u ≃ t)
-  | Trans Γ t u v : Γ ⊢ (t ≃ u) → Γ ⊢ (u ≃ v) → Γ ⊢ (t ≃ v)
+/-- Definition for derivability -/
+inductive derive.{u} {α : Type u} (Γ : Ctx α) : MagmaLaw α → Type u :=
+  | Ax {E} (h : E ∈ Γ) : Γ ⊢ E
+  | Ref {t} : Γ ⊢ t ≃ t
+  | Sym {t u} : Γ ⊢ t ≃ u → Γ ⊢ u ≃ t
+  | Trans {t u v} : Γ ⊢ t ≃ u → Γ ⊢ u ≃ v → Γ ⊢ t ≃ v
   -- This is not as polymorphic as it could be, shouldn't be an issue at the moment
-  | Subst Γ t u σ : Γ ⊢ (t ≃ u) → Γ ⊢ (t ⬝ σ ≃ u ⬝ σ)
-  | Cong Γ t₁ t₂ u₁ u₂ : Γ ⊢ (t₁ ≃ t₂) → Γ ⊢ (u₁ ≃ u₂) → Γ ⊢ (t₁ ⋆ u₁ ≃ t₂ ⋆ u₂)
+  | Subst {t u} σ : Γ ⊢ t ≃ u → Γ ⊢ evalInMagma σ t ≃ evalInMagma σ u
+  | Cong {t₁ t₂ u₁ u₂} : Γ ⊢ (t₁ ≃ t₂) → Γ ⊢ (u₁ ≃ u₂) → Γ ⊢ (t₁ ⋆ u₁ ≃ t₂ ⋆ u₂)
 
 local infix:50 " ⊢' " =>  derive'
 
 /-- Definition for derivability where Subst can only be applied to Ax -/
-inductive derive' {α} : Ctx α → MagmaLaw α → Type :=
-  | SubstAx Γ E (h : E ∈ Γ) σ : Γ ⊢' E.lhs ⬝ σ ≃ E.rhs ⬝ σ
-  | Ref Γ t : Γ ⊢' (t ≃ t)
-  | Sym Γ t u : Γ ⊢' (t ≃ u) → Γ ⊢' (u ≃ t)
-  | Trans Γ t u v : Γ ⊢' (t ≃ u) → Γ ⊢' (u ≃ v) → Γ ⊢' (t ≃ v)
-  | Cong Γ t₁ t₂ u₁ u₂ : Γ ⊢' (t₁ ≃ t₂) → Γ ⊢' (u₁ ≃ u₂) → Γ ⊢' (t₁ ⋆ u₁ ≃ t₂ ⋆ u₂)
+inductive derive'.{u, v} {α : Type u} {β : Type v} (Γ : Ctx α) : MagmaLaw β → Type (max u v) :=
+  | SubstAx {E} (h : E ∈ Γ) (σ) : Γ ⊢' evalInMagma σ E.lhs ≃ evalInMagma σ E.rhs
+  | Ref {t} : Γ ⊢' t ≃ t
+  | Sym {t u} : Γ ⊢' t ≃ u → Γ ⊢' u ≃ t
+  | Trans {t u v} : Γ ⊢' t ≃ u → Γ ⊢' u ≃ v → Γ ⊢' t ≃ v
+  | Cong {t₁ t₂ u₁ u₂} : Γ ⊢' t₁ ≃ t₂ → Γ ⊢' u₁ ≃ u₂ → Γ ⊢' t₁ ⋆ u₁ ≃ t₂ ⋆ u₂
 
-def derive_of_derive' {α} {Γ: Ctx α} {E : MagmaLaw α} : Γ ⊢' E → Γ ⊢ E
-  | .SubstAx _ E h σ => derive.Subst Γ E.lhs E.rhs σ (derive.Ax Γ E h)
-  | .Ref _ t => derive.Ref Γ t
-  | .Sym _ t u h => derive.Sym Γ t u (derive_of_derive' h)
-  | .Trans _ t u v htu huv => derive.Trans Γ t u v (derive_of_derive' htu) (derive_of_derive' huv)
-  | .Cong _ t₁ t₂ u₁ u₂ h₁ h₂ => derive.Cong Γ t₁ t₂ u₁ u₂ (derive_of_derive' h₁) (derive_of_derive' h₂)
+def derive_of_derive' {α} {Γ : Ctx α} {E : MagmaLaw α} : Γ ⊢' E → Γ ⊢ E
+  | .SubstAx (E := E) h σ => derive.Subst σ (derive.Ax h)
+  | .Ref  => derive.Ref
+  | .Sym h => derive.Sym (derive_of_derive' h)
+  | .Trans htu huv => derive.Trans (derive_of_derive' htu) (derive_of_derive' huv)
+  | .Cong h₁ h₂ => derive.Cong (derive_of_derive' h₁) (derive_of_derive' h₂)
+
+def derive'_of_derive {α} {Γ : Ctx α} {E : MagmaLaw α} (H : Γ ⊢ E) : Γ ⊢' E := by
+  simpa [evalInMagma_leaf] using go Lf H
+where
+  go {β} (σ : α → FreeMagma β) {E} : Γ ⊢ E → Γ ⊢' evalInMagma σ E.lhs ≃ evalInMagma σ E.rhs
+  | .Ax h => derive'.SubstAx h σ
+  | .Ref  => .Ref
+  | .Sym h => .Sym (go σ h)
+  | .Trans htu huv => .Trans (go σ htu :) (go σ huv)
+  | .Subst σ h => by simpa [SubstEval] using go _ h
+  | .Cong h₁ h₂ => .Cong (go σ h₁) (go σ h₂)
 
 end DeriveDef
 
 /-- Definitions of entailment -/
-def satisfiesPhi {α G : Type} [Magma G] (φ : α → G) (E : MagmaLaw α) : Prop :=
+def satisfiesPhi {α G} [Magma G] (φ : α → G) (E : MagmaLaw α) : Prop :=
   E.lhs.evalInMagma φ = E.rhs.evalInMagma φ
 
-def satisfies {α : Type} (G : Type) [Magma G] (E : MagmaLaw α) := ∀ (φ : α → G), satisfiesPhi φ E
+/-- `satisfies G E`, or `G ⊧ E`, means that all evaluations of `E` in `G` are true. -/
+def satisfies {α} (G) [Magma G] (E : MagmaLaw α) := ∀ (φ : α → G), satisfiesPhi φ E
 
-def satisfiesSet {α : Type} (G : Type) [Magma G] (Γ : Set (MagmaLaw α)) : Prop :=
+/-- `satisfiesSet G Γ`, or `G ⊧ Γ`, means that `G` satisfies every element of `Γ`. -/
+def satisfiesSet {α} (G) [Magma G] (Γ : Ctx α) : Prop :=
   ∀ E ∈ Γ, satisfies G E
 
-def models {α} (Γ : Ctx α) (E : MagmaLaw α) : Prop :=
-  ∀ (G : Type)[Magma G], satisfiesSet G Γ → satisfies G E
+/-- `models Γ E`, or `Γ ⊧ E`, means that every magma `G` satisfying `Γ` also satisfies `E`. -/
+def models {α β} (Γ : Ctx α) (E : MagmaLaw β) : Prop :=
+  ∀ (G : Type) [Magma G], satisfiesSet G Γ → satisfies G E
 
-/-- Notation for derivability and entailment -/
-infix:50 " ⊧ " => (satisfies)
+/-! Notation for derivability and entailment -/
 
-infix:50 " ⊧ " => (satisfiesSet)
+@[inherit_doc] infix:50 " ⊧ " => satisfies
 
-infix:50 " ⊧ " => (models)
+@[inherit_doc] infix:50 " ⊧ " => satisfiesSet
 
-infix:50 " ⊢ " => (derive)
+@[inherit_doc] infix:50 " ⊧ " => models
 
-infix:50 " ⊢' " => (derive')
+@[inherit_doc] infix:50 " ⊢ " => derive
+
+@[inherit_doc] infix:50 " ⊢' " => derive'
 
 namespace Law
 
-def MagmaLaw.symm {α : Type} (l : MagmaLaw α) : MagmaLaw α := {lhs := l.rhs, rhs:=l.lhs}
+namespace MagmaLaw
+
+def symm {α} (l : MagmaLaw α) : MagmaLaw α := {lhs := l.rhs, rhs:=l.lhs}
 
 @[simp]
-theorem MagmaLaw.symm_symm {α : Type} (l : MagmaLaw α) : l.symm.symm = l := by
+theorem symm_symm {α} (l : MagmaLaw α) : l.symm.symm = l := by
   simp [symm]
 
-theorem satisfiesPhi_symm_law {α G : Type} [Magma G] (φ : α → G) (E : MagmaLaw α)
+def map {α β} (f : α → β) : MagmaLaw α → MagmaLaw β
+  | ⟨lhs, rhs⟩ => ⟨fmapHom f lhs, fmapHom f rhs⟩
+
+theorem map_id {α} (m : MagmaLaw α) : m.map id = m := by
+  simp [map, fmapHom_id]
+
+theorem map_comp {α β γ} (f : α → β) (g : β → γ) (m : MagmaLaw α) :
+    (m.map f).map g = m.map (g ∘ f) := by
+  simp [map, fmapHom_comp']
+
+def Mem {α} (a : α) (m : MagmaLaw α) : Prop :=
+  m.lhs.Mem a ∨ m.rhs.Mem a
+
+def elems {α} [DecidableEq α] (m : MagmaLaw α) :
+    {l : List α // l.Nodup ∧ ∀ a, a ∈ l ↔ Mem a m} := by
+  let ⟨l, _, hl⟩ := m.lhs.elems
+  let ⟨r, nr, hr⟩ := m.rhs.elems
+  use l ∪ r, .union _ nr; simp [Mem, hl, hr]
+
+instance {α} [DecidableEq α] (a : α) (m : MagmaLaw α) : Decidable (Mem a m) :=
+  decidable_of_iff _ (m.elems.2.2 _)
+
+def finEquiv {α} [DecidableEq α] (m : MagmaLaw α) : Fin m.elems.1.length ≃ {a // Mem a m} := by
+  convert ← m.elems.2.1.getEquiv; apply m.elems.2.2
+
+def pmap {α β} : ∀ (m : MagmaLaw α), (∀ a, Mem a m → β) → MagmaLaw β
+  | ⟨lhs, rhs⟩, f =>
+    ⟨lhs.pmap fun a h => f a (.inl h), rhs.pmap fun a h => f a (.inr h)⟩
+
+def attach {α} (m : MagmaLaw α) : MagmaLaw {a // Mem a m} := pmap m .mk
+
+theorem attach_map_val {α} (m : MagmaLaw α) : m.attach.map (·.val) = m := by
+  apply congrArg₂ MagmaLaw.mk <;> exact (evalInMagma_pmap _ (by simp)).trans (fmapHom_id _)
+
+def toFin {α} [DecidableEq α] (m : MagmaLaw α) : MagmaLaw (Fin m.elems.1.length) :=
+  m.attach.map (finEquiv m).symm
+
+def toNat {α} [DecidableEq α] (m : MagmaLaw α) : MagmaLaw ℕ :=
+  (toFin m).map (·.val)
+
+theorem pmap_eq_map {α β} (m : MagmaLaw α)
+    (f : (a : α) → Mem a m → β) (g : α → β) (h : ∀ a h, f a h = g a) :
+    m.pmap f = m.map g := by
+  simp [pmap, FreeMagma.pmap, map]; constructor <;> (apply FreeMagma.pmap_eq_map; intros; apply h)
+
+end MagmaLaw
+
+theorem satisfiesPhi_symm_law {α G} [Magma G] (φ : α → G) (E : MagmaLaw α)
     (h : satisfiesPhi φ E) : satisfiesPhi φ E.symm := by
   simp only [satisfiesPhi, MagmaLaw.symm]; exact h.symm
 
-theorem satisfiesPhi_symm {α G : Type} [Magma G] (φ : α → G) (w₁ w₂ : FreeMagma α)
+theorem satisfiesPhi_map {α β G} [Magma G] {φ : β → G} {f : α → β} {E : MagmaLaw α} :
+    satisfiesPhi φ (E.map f) ↔ satisfiesPhi (φ ∘ f) E := by
+  simp [satisfiesPhi, MagmaLaw.map, evalInMagma_fmapHom]
+
+theorem satisfiesPhi_pmap {α β G} [Magma G] {φ : β → G} {ψ : α → G}
+    (E : MagmaLaw α) (f : (a : α) → E.Mem a → β) (H : ∀ a h, φ (f a h) = ψ a) :
+    satisfiesPhi φ (E.pmap f) ↔ satisfiesPhi ψ E := by
+  simp [satisfiesPhi, MagmaLaw.pmap]
+  rw [evalInMagma_pmap _ fun a h => H a (.inl h),
+      evalInMagma_pmap _ fun a h => H a (.inr h)]
+
+theorem satisfiesPhi_attach {α G} [Magma G] {φ : α → G} {E : MagmaLaw α} :
+    satisfiesPhi (φ ·.1) E.attach ↔ satisfiesPhi φ E := by
+  apply satisfiesPhi_pmap; intros; rfl
+
+theorem satisfiesPhi_symm {α G} [Magma G] (φ : α → G) (w₁ w₂ : FreeMagma α)
     (h : satisfiesPhi φ (w₁ ≃ w₂)) : satisfiesPhi φ (w₂ ≃ w₁) :=
   Law.satisfiesPhi_symm_law φ (w₁ ≃ w₂) h
 
-theorem satisfies_symm_law {α : Type} (G : Type) [Magma G] (E : MagmaLaw α) (h : G ⊧ E) :
+theorem equiv_satisfiesPhi {α G H} [Magma G] [Magma H] {φ : α → G} (e : G ≃◇ H) {E : MagmaLaw α} :
+    satisfiesPhi (e ∘ φ) E ↔ satisfiesPhi φ E := by
+  simp [satisfiesPhi, ← evalInMagma_equiv]
+
+theorem satisfies_symm_law {α G} [Magma G] {E : MagmaLaw α} (h : G ⊧ E) :
     G ⊧ E.symm :=
   fun φ ↦ satisfiesPhi_symm_law φ E (h φ)
 
-theorem satisfies_symm {α : Type} (G : Type) [Magma G] (w₁ w₂ : FreeMagma α) (h : G ⊧ w₁ ≃ w₂) :
+theorem satisfies_map {α β G} [Magma G] (f : α → β) {E : MagmaLaw α} (h : G ⊧ E) :
+    G ⊧ E.map f := fun _ ↦ satisfiesPhi_map.2 (h _)
+
+theorem satisfies_map_injective {α β G} [Magma G] (f : α → β) (hf : f.Injective) {E : MagmaLaw α} :
+    G ⊧ E.map f ↔ G ⊧ E := by
+  refine ⟨fun H φ => ?_, satisfies_map _⟩
+  have : Inhabited α := ⟨E.lhs.first⟩
+  have ⟨g, hg⟩ := hf.hasLeftInverse
+  rw [← MagmaLaw.map_id E, ← show g ∘ f = id from funext hg, ← MagmaLaw.map_comp, satisfiesPhi_map]
+  apply H
+
+theorem satisfies_map_equiv {α β G} [Magma G] (f : α ≃ β) {E : MagmaLaw α} :
+    G ⊧ E.map f ↔ G ⊧ E := satisfies_map_injective _ f.injective
+
+theorem satisfies_attach {α G} [DecidableEq α] [Magma G] {E : MagmaLaw α} :
+    G ⊧ E.attach ↔ G ⊧ E := by
+  refine ⟨fun h φ => satisfiesPhi_attach.1 (h _), fun h φ => ?_⟩
+  have : Inhabited G := ⟨φ ⟨E.lhs.first, .inl E.lhs.first_mem⟩⟩
+  let ψ a := if h : E.Mem a then φ ⟨a, h⟩ else default
+  exact (satisfiesPhi_pmap (ψ := ψ) _ _ (fun a h => by simp [ψ, h])).2 (h _)
+
+theorem satisfies_toFin {α G} [DecidableEq α] [Magma G] {E : MagmaLaw α} :
+    G ⊧ E.toFin ↔ G ⊧ E :=
+  (satisfies_map_equiv _).trans satisfies_attach
+
+theorem satisfies_toNat {α G} [DecidableEq α] [Magma G] {E : MagmaLaw α} :
+    G ⊧ E.toNat ↔ G ⊧ E :=
+  (satisfies_map_injective _ Fin.val_injective).trans satisfies_toFin
+
+theorem satisfies_symm {α G} [Magma G] {w₁ w₂ : FreeMagma α} (h : G ⊧ w₁ ≃ w₂) :
     G ⊧ w₂ ≃ w₁ :=
-  satisfies_symm_law G (w₁ ≃ w₂) h
+  satisfies_symm_law h
 
-def set_symm {α} (Γ : Set (MagmaLaw α)) : Set (MagmaLaw α) := { (γ.symm) | γ ∈ Γ}
+theorem satisfies_equiv {α G H} [Magma G] [Magma H] (e : G ≃◇ H) {E : MagmaLaw α} :
+    G ⊧ E ↔ H ⊧ E := by
+  constructor <;> intro h φ
+  · rw [← equiv_satisfiesPhi e.symm]; apply h
+  · rw [← equiv_satisfiesPhi e]; apply h
 
-theorem satisfiesSet_symm {α : Type} (G : Type) [Magma G] (Γ : Set (MagmaLaw α))
-  (h :  G ⊧ Γ) : G ⊧ (set_symm Γ) :=
-  fun _ ⟨_, ⟨hEsymm, hEsymmE⟩⟩ ↦ hEsymmE ▸ Law.satisfies_symm _ _ _ (h _ hEsymm)
+theorem satisfiesSet_symm {α G} [Magma G] {Γ : Ctx α}
+  (h :  G ⊧ Γ) : G ⊧ (·.symm) '' Γ :=
+  fun _ ⟨_, ⟨hEsymm, hEsymmE⟩⟩ ↦ hEsymmE ▸ Law.satisfies_symm (h _ hEsymm)
 
-theorem models_symm_law {α} (Γ : Ctx α) (E : MagmaLaw α) (h : Γ ⊧ E) : Γ   ⊧ E.symm :=
-  fun G [Magma G] hsatisfiesSet ↦ satisfies_symm_law G E (h G hsatisfiesSet)
+theorem satisfiesSet_equiv {α G H} [Magma G] [Magma H] (e : G ≃◇ H) {Γ : Ctx α} :
+    G ⊧ Γ ↔ H ⊧ Γ :=
+  forall_congr' fun _ => forall_congr' fun _ => satisfies_equiv e
+
+theorem satisfiesSet_toNat {α G} [DecidableEq α] [Magma G] {Γ : Ctx α} :
+    G ⊧ (·.toNat) '' Γ ↔ G ⊧ Γ :=
+  ⟨fun H _ h => satisfies_toNat.1 (H _ ⟨_, h, rfl⟩),
+   fun | H, _, ⟨_, h, rfl⟩ => satisfies_toNat.2 (H _ h)⟩
+
+theorem models_symm_law {α} {Γ : Ctx α} {E : MagmaLaw α} (h : Γ ⊧ E) : Γ ⊧ E.symm :=
+  fun G [Magma G] hsatisfiesSet ↦ satisfies_symm_law (h G hsatisfiesSet)
 
 theorem models_symm {α} (Γ : Ctx α) (w₁ w₂ : FreeMagma α) (h : Γ ⊧ w₁ ≃ w₂) : Γ ⊧ w₂ ≃ w₁ :=
-  Law.models_symm_law Γ (w₁ ≃ w₂) h
+  Law.models_symm_law h
+
+theorem models_toNat {α β} [DecidableEq β] {Γ : Ctx α} {E : MagmaLaw β} :
+    Γ ⊧ E.toNat ↔ Γ ⊧ E :=
+  forall_congr' fun _ => forall_congr' fun _ => imp_congr_right fun _ => satisfies_toNat
+
+theorem toNat_models {α β} [DecidableEq α] {Γ : Ctx α} {E : MagmaLaw β} :
+    (·.toNat) '' Γ ⊧ E ↔ Γ ⊧ E :=
+  forall_congr' fun _ => forall_congr' fun _ => imp_congr_left satisfiesSet_toNat
+
+def derive'_map {α β γ} {f : β → γ} : ∀ {Γ : Ctx α} {E : MagmaLaw β}, Γ ⊢' E → Γ ⊢' E.map f
+  | _, _, .SubstAx h σ => by simp [MagmaLaw.map, evalInMagma_hom]; exact .SubstAx h _
+  | _, _, .Ref => .Ref
+  | _, _, .Sym h => .Sym (derive'_map h)
+  | _, _, .Trans h1 h2 => .Trans (derive'_map h1) (derive'_map h2)
+  | _, _, .Cong h1 h2 => .Cong (derive'_map h1) (derive'_map h2)
+
+theorem derive'_map_injective {α β γ} {f : β → γ} (hf : f.Injective) {Γ : Ctx α} {E : MagmaLaw β} :
+    Nonempty (Γ ⊢' E.map f) ↔ Nonempty (Γ ⊢' E) := by
+  refine ⟨fun ⟨h⟩ => ?_, fun ⟨h⟩ => ⟨derive'_map h⟩⟩
+  have : Inhabited β := ⟨E.lhs.first⟩
+  have ⟨g, hg⟩ := hf.hasLeftInverse
+  rw [← MagmaLaw.map_id E, ← show g ∘ f = id from funext hg, ← MagmaLaw.map_comp]
+  exact ⟨derive'_map h⟩
+
+def derive'_pmap {α β γ} [DecidableEq β] {Γ : Ctx α} {E : MagmaLaw β} (f : ∀ a, E.Mem a → γ) :
+    Γ ⊢' E → Γ ⊢' E.pmap f := by
+  have : Inhabited γ := ⟨f _ (.inl (first_mem _))⟩
+  let k a := if h : _ then f a h else default
+  rw [MagmaLaw.pmap_eq_map E f k fun a h => by simp [k, h]]
+  apply derive'_map
+
+def derive'_attach {α β} [DecidableEq β] {Γ : Ctx α} {E : MagmaLaw β} :
+    Γ ⊢' E → Γ ⊢' E.attach := derive'_pmap _
+
+theorem derive'_attach_iff {α β} [DecidableEq β] {Γ : Ctx α} {E : MagmaLaw β} :
+    Nonempty (Γ ⊢' E.attach) ↔ Nonempty (Γ ⊢' E) :=
+  ⟨fun ⟨h⟩ => ⟨(MagmaLaw.attach_map_val _ ▸ derive'_map h :)⟩, fun ⟨h⟩ => ⟨derive'_attach h⟩⟩
+
+theorem derive'_toFin_iff {α β} [DecidableEq β] {Γ : Ctx α} {E : MagmaLaw β} :
+    Nonempty (Γ ⊢' E.toFin) ↔ Nonempty (Γ ⊢' E) :=
+  (derive'_map_injective (Equiv.injective _)).trans derive'_attach_iff
+
+theorem derive'_toNat_iff {α β} [DecidableEq β] {Γ : Ctx α} {E : MagmaLaw β} :
+    Nonempty (Γ ⊢' E.toNat) ↔ Nonempty (Γ ⊢' E) :=
+  (derive'_map_injective Fin.val_injective).trans derive'_toFin_iff
 
 end Law
